Work in progress

hello.fst
@@ -1,5 +1,5 @@
 (*--build-config
-options:--admit_fsi FStar.Set --admit_fsi FStar.Heap --admit_fsi FStar.ST --admit_fsi FStar.All --admit_fsi FStar.IO;
+options:--n_cores 2 --max_fuel 2 --admit_fsi FStar.Set --admit_fsi FStar.Heap --admit_fsi FStar.ST --admit_fsi FStar.All --admit_fsi FStar.IO;
 other-files:set.fsi heap.fst st.fst all.fst io.fsti string.fst listTot.fst char.fst terminal.fst;
 --*)
 module Hello
@@ -31,22 +31,31 @@ type editorChar = (char * bool)
 val pad_line : nat -> list editorChar -> Tot (list editorChar)
 let pad_line n cs = pad_list n (' ',false) cs
 
+val hdcons : 'a -> xss:list (list 'a){xss<>[]} -> yss:list (list 'a){yss<>[]}
+let hdcons x xss = (x::hd xss)::tl xss
+
+val listSplit : ('a -> Tot bool) -> list 'a -> Tot (yss:list (list 'a){yss<>[]})
+let rec listSplit p xs' = match xs' with
+  | [] -> [[]]
+  | x::xs -> let yss = listSplit p xs in
+    if p x then
+      [x]::yss
+    else
+      hdcons x yss
+
 val isLineBreak : editorChar -> Tot bool
 let isLineBreak (ch,_) = (ch = '\n')
 
-val listLines : list editorChar -> Tot (list editorChar * list (list editorChar))
-let rec listLines cs' = match cs' with
-  | [] -> ([],[])
-  | c::cs -> let (line,lines) = listLines cs in
-    if isLineBreak c then
-      ([c], line :: lines)
-    else
-      (c::line, lines)
+val listLines : list editorChar -> Tot (list (list editorChar))
+let listLines es = listSplit isLineBreak es
 
 val annotate : list char -> int -> Tot (list editorChar)
 let rec annotate cs' n = match cs' with
   | [] -> []
   | c::cs -> (c,n=0)::annotate cs (n-1)
+
+val buffer_annotate : buffer -> Tot (list editorChar)
+let buffer_annotate (w,h,pos,str) = annotate str pos
 
 val scrubCursor : list (list editorChar) -> Tot (list (list char))
 let scrubCursor = map (map fst)
@@ -73,30 +82,37 @@ let findCursorOrZero ess = match findCursor ess with
   | None -> (0,0)
   | Some (m,n) -> (m,n)
 
+val buffer_lines : buffer -> Tot (list (list editorChar))
+let buffer_lines buf = listLines (buffer_annotate buf)
+
+val buffer_w : buffer -> Tot nat
+let buffer_w (w, _, _, _) = w
+
+val buffer_h : buffer -> Tot nat
+let buffer_h (_, h, _, _) = h
+
+val buffer_pos : buffer -> Tot nat
+let buffer_pos (_, _, pos, _) = pos
+
+val buffer_cs : buffer -> Tot (list char)
+let buffer_cs (_, _, _, cs) = cs
+
+val buffer_padded_lines : buffer -> Tot (list (list editorChar))
+let buffer_padded_lines buf = map (fun line -> pad_line (buffer_w buf) line) (buffer_lines buf)
+
 val display_buffer : buffer -> Tot terminalScreen
-let display_buffer (w, h, pos, bufstr) =
-  let echars = annotate bufstr pos in
-  let (line,lines) = listLines echars in
-  let lines' = line::lines in
-  let padded_lines = map (fun line -> pad_line w line) lines' in
+let display_buffer buf =
+  let w = buffer_w buf in
+  let h = buffer_h buf in
+  let padded_lines = buffer_padded_lines buf in
   let empty_line = pad_line w [] in
   let egrid = pad_list h empty_line padded_lines in
   let grid = scrubCursor egrid in
   let (cx,cy) = findCursorOrZero egrid in
   Screen w h cx cy grid
 
-type buffer_changer b =
-  p:(buffer * list char){Some (display_buffer (fst p)) = screen_advance (snd p) (display_buffer b)}
-//type buffer_changer (b:buffer) = (buffer * list char)
-
-//val l_screen_advance_empty : (s:terminalScreen) -> Lemma (screen_advance [] s = Some s)
-//let l_screen_advance_empty b = ()
-
 val state : ref buffer
 let state = ST.alloc (80,25,0,[])
-
-val noop : b:buffer -> Tot (buffer_changer b)
-let noop buf = (buf,[])
 
 val list_insert : nat -> 'a -> list 'a -> Tot (list 'a)
 let rec list_insert i y xs' =
@@ -106,11 +122,221 @@ let rec list_insert i y xs' =
     | [] -> [y]
     | x::xs -> x::list_insert (i-1) y xs
 
-val insert_char : char -> b:buffer -> Tot (buffer_changer b)
-let insert_char ch (w,h,i,chars) =
+type buffer_changer b =
+  p:(buffer * list char){Some (display_buffer (fst p)) = screen_advance (snd p) (display_buffer b)}
+//type buffer_changer (b:buffer) = (buffer * list char)
+
+val noop : b:buffer -> Tot (buffer_changer b)
+let noop buf = (buf,[])
+
+val buffer_insert : char -> buffer -> Tot buffer
+let buffer_insert ch (w,h,i,chars) =
   let chars' = list_insert i ch chars in
-  let buf' = (w,h,i+1,chars') in
+  (w,h,i+1,chars')
+
+(* The effect that inserting a character has on annotate *)
+val annotate_ins_empty : n:nat -> ch:char -> Lemma (annotate (list_insert n ch []) (n+1) = list_insert n (ch,false) (annotate [] n))
+let annotate_ins_empty n ch = ()
+
+val annotate_ins :
+  n:nat -> cs:list char -> ch:char ->
+  Lemma (annotate (list_insert n ch cs) (n+1)
+    = list_insert n (ch,false) (annotate cs n))
+let rec annotate_ins n cs' ch =
+  match cs' with
+  | [] -> annotate_ins_empty n ch
+  | c::cs -> match n with
+    | 0 -> ()
+    | _ -> annotate_ins (n-1) cs ch
+
+val buffer_annotate_ins :
+  b:buffer -> ch:char ->
+  Lemma (buffer_annotate (buffer_insert ch b)
+    = list_insert (buffer_pos b) (ch,false) (buffer_annotate b))
+let buffer_annotate_ins b ch
+  = annotate_ins (buffer_pos b) (buffer_cs b) ch
+
+val grow_char : char -> editorChar -> Tot (list editorChar)
+let grow_char ch (c,cursor) = if cursor then [(ch,false);(c,cursor)] else [(c,cursor)]
+
+val line_insert : char -> list editorChar -> Tot (list editorChar)
+let line_insert ch es = concatMap (grow_char ch) es
+
+val lines_insert : char -> list (list editorChar) -> Tot (list (list editorChar))
+let lines_insert ch b = map (line_insert ch) b
+
+(* The effect of inserting a character into appended lines *)
+val line_ins_append : ch:char -> es:list editorChar -> ess:list (list editorChar) ->
+  Lemma (lines_insert ch (es::ess) = line_insert ch es::lines_insert ch ess)
+let line_ins_append ch es ess = ()
+
+(*
+val has_no_linebreaks : list editorChar -> Tot bool
+let rec has_no_linebreaks es' = match es' with
+  | [] -> true
+  | e::es -> not(isLineBreak e) && has_no_linebreaks es
+
+val only_has_linebreak_at_end : list editorChar -> Tot bool
+let rec only_has_linebreak_at_end es' = match es' with
+  | [] -> false
+  | [e] -> isLineBreak e
+  | e::f::es -> not(isLineBreak e) && only_has_linebreak_at_end (f::es)
+
+val grow_no_linebreaks : ch:char{ch<>'\n'} -> e:editorChar{not(isLineBreak e)} ->
+  Lemma (has_no_linebreaks (grow_char ch e))
+let grow_no_linebreaks ch (c,b) =
+  if b then (
+    assert(grow_char ch (c,b) = [(ch,false);(c,b)]);
+    assert(has_no_linebreaks [(c,b)]);
+    assert(not(isLineBreak((ch,false))));
+    assert(has_no_linebreaks([(ch,false);(c,b)]));
+    ()
+  ) else (
+    assert(grow_char ch (c,b) = [(c,b)]);
+    ()
+  )
+  
+val grow_only_linebreak_at_end : ch:char{ch<>'\n'} -> e:editorChar{isLineBreak e} ->
+  Lemma (only_has_linebreak_at_end (grow_char ch e))
+let grow_only_linebreak_at_end ch (c,b) =
+  if b then (
+    assert(grow_char ch (c,b) = [(ch,false);(c,b)]);
+    ()
+  ) else (
+    assert(grow_char ch (c,b) = [(c,b)]);
+    ()
+  )
+
+(* Appending a has_no_linebreaks *)
+val appending_no_linebreaks : es:list editorChar{has_no_linebreaks es} -> fs:list editorChar ->
+  Lemma (listLines (es @@ fs) = (es @@ hd (listLines fs)) :: tl (listLines fs))
+let rec appending_no_linebreaks es' fs =
+  match es' with
+    | [] -> ()
+    | (e::es) ->
+      assert(not(isLineBreak e));
+      //assert listLines ((e::es)@fs) = (e::hd (listLines (es@@fs)))::tl (listLines (es@@fs))
+      appending_no_linebreaks es fs;
+      ()
+
+(* Appending only_has_linebreak_at_end *)
+val appending_only_linebreak_at_end : es:list editorChar{only_has_linebreak_at_end es} -> fs:list editorChar ->
+  Lemma (listLines (es @@ fs) = es :: listLines fs)
+let rec appending_only_linebreak_at_end es' fs =
+  match es' with
+    | [] -> assert(false)
+    | [e] ->
+      assert(isLineBreak e);
+      ()
+    | e::e'::es ->
+      assert(not(isLineBreak e));
+      appending_only_linebreak_at_end (e'::es) fs;
+      ()
+*)
+
+val listLines_cons : e:editorChar{~isLineBreak e} -> es:list editorChar ->
+  Lemma (listLines (e::es) = hdcons e (listLines es))
+let listLines_cons e es = ()
+
+val lines_ins_linebreak : e:editorChar{isLineBreak e} -> es:list editorChar -> ch:char{isPrintableChar ch} ->
+  Lemma (listLines (line_insert ch (e::es)) = lines_insert ch (listLines (e::es)))
+let lines_ins_linebreak :
+	assert(not(isLineBreak (ch,false)));
+	assert(isLineBreak e);
+	grow_only_linebreak_at_end ch e;
+        assert(only_has_linebreak_at_end (grow_char ch e));
+	lines_ins es ch;
+	line_ins_append ch [e] (listLines es);
+        assert(line_insert ch (e::es) = (grow_char ch e @@ line_insert ch es));
+	appending_only_linebreak_at_end (grow_char ch e) (line_insert ch es);
+	assert(listLines (line_insert ch (e::es)) = listLines (grow_char ch e @@ line_insert ch es));
+	assert(listLines (line_insert ch (e::es)) = lines_insert ch (listLines (e::es)));
+	assert(listLines (line_insert ch es') = lines_insert ch (listLines es'))
+
+(* The effect that inserting a character has on lines *)
+val lines_ins : es:list editorChar -> ch:char{isPrintableChar ch} ->
+  Lemma (listLines (line_insert ch es) = lines_insert ch (listLines es))
+let rec lines_ins es' ch =
+  (match es' with
+    | [] -> ()
+    | e::es ->
+      if isLineBreak e then (
+      ) else (
+	assert(not(isLineBreak (ch,false)));
+	assert(not(isLineBreak e));
+	grow_no_linebreaks ch e;
+        assert(has_no_linebreaks (grow_char ch e));
+        lines_ins es ch;
+	line_ins_append ch (e::hd (listLines es)) (tl (listLines es));
+	appending_no_linebreaks (grow_char ch e) (line_insert ch es);
+	assert(listLines (line_insert ch (e::es)) = lines_insert ch (listLines (e::es)));
+	assert(listLines (line_insert ch es') = lines_insert ch (listLines es'))
+      );
+      assert(listLines (line_insert ch es') = lines_insert ch (listLines es'))
+  );
+  assert(listLines (line_insert ch es') = lines_insert ch (listLines es'))
+  
+val line_insert_annotate_negative : es:list char -> n:int{n<0} -> ch:char ->
+  Lemma (line_insert ch (annotate es n) = annotate es n)
+let rec line_insert_annotate_negative es' n ch = match es' with
+  | [] -> ()
+  | e::es -> line_insert_annotate_negative es (n-1) ch
+
+val list_insert_line_insert0 : c:char -> cs:list char -> ch:char ->
+  Lemma (list_insert 0 (ch,false) (annotate (c::cs) 0) = line_insert ch (annotate (c::cs) 0))
+let list_insert_line_insert0 c cs ch =
+      assert(list_insert 0 (ch,false) (annotate (c::cs) 0) = (ch,false)::annotate (c::cs) 0);
+      assert(annotate (c::cs) 0 = (c,true)::annotate cs (-1));
+      line_insert_annotate_negative cs (-1) ch;
+      assert(line_insert ch (annotate (c::cs) 0) = (ch,false)::annotate (c::cs) 0);
+      ()
+
+val list_insert_line_insert' : es:list char -> n:nat -> ch:char ->
+  Lemma (list_insert n (ch,false) (annotate es n) = line_insert ch (annotate es n))
+let rec list_insert_line_insert' es' n ch
+  = match es' with
+  | [] -> ()
+  | e::es ->
+    match n with
+    | 0 ->
+       list_insert_line_insert0 e es ch
+    | _ ->
+      list_insert_line_insert' es (n-1) ch;
+      assert(list_insert n (ch,false) (annotate es' n) = line_insert ch (annotate es' n));
+      ()
+
+(*val list_insert_line_insert : b:buffer -> ch:char ->
+  Lemma (list_insert (buffer_pos b) (ch,false) (buffer_annotate b) = line_insert ch (buffer_annotate b))
+let rec list_insert_line_insert (w,h,pos,cs') ch
+  = match cs' with
+  | [] -> ()
+  | c::cs ->
+      match pos with
+      | 0 ->
+	assert(buffer_annotate (w,h,pos,cs') = *)
+
+val buffer_lines_ins : b:buffer -> ch:char{isPrintableChar ch} ->
+  Lemma (buffer_lines (buffer_insert ch b) = lines_insert ch (buffer_lines b))
+let buffer_lines_ins b ch =
+  assert(buffer_lines (buffer_insert ch b) = listLines (buffer_annotate (buffer_insert ch b)));
+  buffer_annotate_ins b ch;
+  list_insert_line_insert' (buffer_cs b) (buffer_pos b) ch;
+  assert (list_insert (buffer_pos b) (ch,false) (buffer_annotate b) = line_insert ch (buffer_annotate b));
+  assert(buffer_annotate (buffer_insert ch b) = line_insert ch (buffer_annotate b));
+  lines_ins (buffer_annotate b) ch
+
+(* The effect that inserting a character has on display_buffer *)
+val buffer_inserting_character :
+  b:buffer -> ch:char{isPrintableChar ch} ->
+  Lemma (display_buffer (buffer_insert ch b)
+    = screenInsertChar ch (display_buffer b))
+let buffer_inserting_character b ch = buffer_annotate_ins b ch
+
+val insert_char : char -> b:buffer -> Tot (buffer_changer b)
+let insert_char ch buf =
+  let buf' = buffer_insert ch buf in
   let output = esc::'['::'@'::ch::[] in
+  buffer_inserting_character buf ch;
   (buf', output)
 
 val handle_key : char -> b:buffer -> Tot (buffer_changer b)
